Introduce a built-in notion of "trace invariant", as in the paper
The specification for Emit now states that one has to respect the
trace invariant

theories/heap_lang/lifting.v
@@ -1,8 +1,9 @@
 From stdpp Require Import fin_maps.
 From iris.proofmode Require Import tactics.
 From iris.algebra Require Import auth excl agree gmap list.
+From iris.algebra.lib Require Import frac_auth.
 From iris.base_logic Require Export gen_heap.
-From iris.base_logic.lib Require Export proph_map.
+From iris.base_logic.lib Require Export proph_map invariants.
 From iris.program_logic Require Export weakestpre total_weakestpre.
 From iris.program_logic Require Import ectx_lifting total_ectx_lifting.
 From intensional Require Export lang.
@@ -38,17 +39,17 @@ Definition traceO := leibnizO (list event).
 Class traceG Σ := TraceG {
   trace_hist_inG :> inG Σ (authR (gmapUR nat (agreeR eventO)));
   trace_hist_name : gname;
-  trace_inG :> inG Σ (authR (optionUR (exclR traceO)));
+  trace_inG :> inG Σ (frac_authR (agreeR traceO));
   trace_name : gname;
 }.
 
 Definition traceΣ : gFunctors :=
-  #[GFunctor (authR (optionUR (exclR traceO)));
-    GFunctor (authR (gmapUR nat (agreeR eventO)))].
+  #[GFunctor (authR (gmapUR nat (agreeR eventO)));
+    GFunctor (frac_authR (agreeR traceO))].
 
 Class trace_preG Σ := TracePreG {
   trace_hist_preG_inG :> inG Σ (authR (gmapUR nat (agreeR eventO)));
-  trace_preG_inG :> inG Σ (authR (optionUR (exclR (leibnizO (list event)))));
+  trace_preG_inG :> inG Σ (frac_authR (agreeR (leibnizO (list event))));
 }.
 
 Instance subG_tracePreG : subG traceΣ Σ → trace_preG Σ.
@@ -62,11 +63,16 @@ Class heapG Σ := HeapG {
 }.
 
 Definition trace_auth `{hT: traceG Σ} (t: list event) :=
-  (own trace_name (● (Excl' (t: traceO))) ∗ own trace_hist_name (● gmap_of_trace 0 t))%I.
+  (own trace_name (●F (to_agree (t: traceO))) ∗ own trace_hist_name (● gmap_of_trace 0 t))%I.
 Definition hist `{hT: traceG Σ} (t: list event) :=
   own trace_hist_name (◯ (gmap_of_trace 0 t)).
+Definition trace_half_frag `{hT:traceG} (t: list event) :=
+  own trace_name (◯F{1/2} (to_agree (t: traceO))).
 Definition trace_is `{hT: traceG Σ} (t: list event) :=
-  (own trace_name (◯ (Excl' (t: traceO))) ∗ hist t)%I.
+  (trace_half_frag t ∗ hist t)%I.
+
+Definition trace_inv `{hT:traceG Σ, hI:invG Σ} (ι: namespace) (I: list event → Prop) :=
+  inv ι (∃ t, trace_half_frag t ∗ ⌜I t⌝).
 
 Instance hist_persistent `{traceG Σ} (t: list event): Persistent (hist t) := _.
 
@@ -77,36 +83,51 @@ Proof.
   iFrame. iSplit; iAssumption.
 Qed.
 
+Lemma trace_auth_half_frag_agree `{traceG Σ} t t':
+  trace_auth t -∗ trace_half_frag t' -∗ ⌜t = t'⌝.
+Proof.
+  rewrite /trace_auth /trace_is.
+  iIntros "[H1 _] H2".
+  iDestruct (own_valid_2 with "H1 H2") as "H".
+  iDestruct "H" as %Hi%frac_auth_included.
+  rewrite -> Some_included_total in Hi.
+  apply to_agree_included, leibniz_equiv in Hi. eauto.
+Qed.
+
 Lemma trace_agree `{traceG Σ} t t':
   trace_auth t -∗ trace_is t' -∗ ⌜t = t'⌝.
 Proof.
-  rewrite /trace_auth /trace_is.
-  iIntros "[H1 _] [H2 _]".
-  iDestruct (own_valid_2 with "H1 H2") as "H".
-  iDestruct "H" as %[Hi%Excl_included _]%auth_both_valid.
-  eapply leibniz_equiv in Hi; eauto.
+  iIntros "H1 [H2 _]". iApply (trace_auth_half_frag_agree with "H1 H2").
 Qed.
 
-Lemma trace_is_excl `{traceG Σ} t t' :
-  trace_is t -∗ trace_is t' -∗ ⌜ False ⌝.
+Lemma trace_half_frag_agree `{traceG Σ} t t':
+  trace_half_frag t -∗ trace_is t' -∗ ⌜t = t'⌝.
 Proof.
-  iIntros "[H1 _] [H2 _]". iDestruct (own_valid_2 with "H1 H2") as %Hv.
-  rewrite -auth_frag_op // in Hv.
+  rewrite /trace_is /trace_half_frag.
+  iIntros "H1 [H2 _]".
+  iDestruct (own_valid_2 with "H1 H2") as "H".
+  rewrite -frac_auth_frag_op Qp_half_half.
+  iDestruct "H" as %Hv. rewrite frac_auth_frag_valid in Hv |- * => Hv.
+  destruct Hv as [_ Hv]. apply agree_op_inv', leibniz_equiv in Hv. eauto.
 Qed.
 
 Lemma trace_add_event `{traceG Σ} t (e: event) :
-  trace_auth t -∗ trace_is t ==∗ trace_auth (t ++ [e]) ∗ trace_is (t ++ [e]).
+  trace_auth t -∗ trace_is t -∗ trace_half_frag t ==∗
+  trace_auth (t ++ [e]) ∗ trace_is (t ++ [e]) ∗ trace_half_frag (t ++ [e]).
 Proof.
   rewrite /trace_auth /trace_is /hist.
-  iIntros "[H1 H1h] [H2 H2h]".
-  iMod (own_update_2 _ _ _ (● Excl' (t++[e]:traceO) ⋅ ◯ Excl' (t++[e]:traceO)) with "H1 H2") as "[? ?]".
-  by apply auth_update, option_local_update, exclusive_local_update.
-  cbn [gmap_of_trace]. rewrite gmap_of_trace_snoc Nat.add_0_l.
+  iIntros "[H1 H1h] [H2 H2h] H3".
+  iDestruct (own_op with "[$H2 $H3]") as "H2".
+  rewrite -frac_auth_frag_op Qp_half_half agree_idemp.
+  iMod (own_update_2 _ _ _ (●F (to_agree (t++[e]:traceO)) ⋅ ◯F (to_agree (t++[e]:traceO))) with "H1 H2") as "[? ?]".
+  by apply frac_auth_update_1.
+  rewrite gmap_of_trace_snoc Nat.add_0_l.
   iMod (own_update_2 with "H1h H2h") as "[? ?]".
   apply auth_update.
   eapply (alloc_local_update _ _ (length t : nat) (to_agree (e:eventO))); [|done].
   { eapply not_elem_of_dom. intros ?%gmap_of_trace_dom. lia. }
   iModIntro. iFrame.
+  rewrite /trace_half_frag -own_op -frac_auth_frag_op Qp_half_half agree_idemp //.
   Unshelve. all: typeclasses eauto.
 Qed.
 
@@ -161,14 +182,17 @@ Proof.
 Qed.
 
 Lemma trace_auth_init `{hT: trace_preG Σ} (t: list event) :
-  ⊢ |==> ∃ H: traceG Σ, trace_auth t.
+  ⊢ |==> ∃ H: traceG Σ, trace_auth t ∗ trace_is t ∗ trace_half_frag t.
 Proof.
-  iMod (own_alloc (● Excl' (t: traceO))) as (γ) "Hγ".
-  by apply auth_auth_valid.
-  iMod (own_alloc (● gmap_of_trace 0 t)) as (γh) "Hγh".
-  apply auth_auth_valid. apply gmap_of_trace_valid.
+  iMod (own_alloc (●F (to_agree (t: traceO)) ⋅ ◯F (to_agree (t: traceO)))) as (γ) "Hγ".
+  by apply frac_auth_valid.
+  rewrite own_op. iDestruct "Hγ" as "[? Hγf]".
+  iMod (own_alloc (● gmap_of_trace 0 t ⋅ ◯ gmap_of_trace 0 t)) as (γh) "Hγh".
+  apply auth_both_valid. split; [ done | by apply gmap_of_trace_valid].
+  rewrite own_op. iDestruct "Hγh" as "[? ?]".
   iModIntro. iExists (TraceG _ _ γh _ γ).
-  rewrite /trace_auth. iFrame.
+  rewrite /trace_auth /trace_is /trace_half_frag /hist. iFrame.
+  rewrite -own_op -frac_auth_frag_op Qp_half_half agree_idemp //.
 Qed.
 
 Instance heapG_irisG `{!heapG Σ} : irisG heap_lang Σ := {
@@ -379,17 +403,25 @@ Implicit Types σ : state.
 Implicit Types v : val.
 Implicit Types l : loc.
 
-Lemma wp_emit s E tr tag v :
-  {{{ trace_is tr }}}
+Lemma wp_emit s E tr tag v ι (I: list event → Prop) :
+  ↑ι ⊆ E →
+  I (tr ++ [(tag, v)]) →
+  {{{ trace_is tr ∗ trace_inv ι I }}}
     Emit tag v @ s; E
   {{{ RET (LitV LitUnit); trace_is (tr ++ [(tag, v)]) }}}.
 Proof.
-  iIntros (φ) "Ht Hφ". iApply wp_lift_atomic_head_step; [done|].
-  iIntros (σ1 κ κs n) "(? & ? & ?) !>"; iSplit; first by eauto.
+  iIntros (Hι HI φ) "[Ht Hi] Hφ".
+  iInv "Hi" as ">Hi" "Hclose".
+  iDestruct "Hi" as (tr') "[Htr' _]".
+  iDestruct (trace_half_frag_agree with "Htr' Ht") as %->.
+  iApply wp_lift_atomic_head_step; [done|].
+  iIntros (σ1 κ κs n) "(? & Hta & ?) !>"; iSplit; first by eauto.
   iNext. iIntros (v2 σ2 efs Hstep); inv_head_step.
-  iDestruct (trace_agree with "[$] [$]") as %?; subst.
-  iMod (trace_add_event with "[$] [$]") as "(?&?)".
-  iModIntro. iFrame. iSplitL; last done. by iApply "Hφ".
+  iDestruct (trace_agree with "Hta Ht") as %<-.
+  iMod (trace_add_event with "Hta Ht Htr'") as "(Hta&Ht&Htr')".
+  iModIntro. iFrame. iSplitL; last done.
+  iMod ("Hclose" with "[Htr']"). { iNext. eauto. }
+  iModIntro. by iApply "Hφ".
 Qed.
 
 (** Fork: Not using Texan triples to avoid some unnecessary [True] *)
